theories/Transition/Temporal/TT_Definition.v
@@ -1,15 +1,29 @@
-From Mecha Require Import Resource Term Typ Var ReadStock WriteStock Stock Typing
-                          Cell VContext REnvironment RContext ET_Definition FT_Definition
-                          Sample Samples.
-(**
+From Mecha Require Import Resource Term ReadStock WriteStock Stock REnvironment
+                          FT_Definition Sample Samples RContext.
+Import ResourceNotations TermNotations StockNotations REnvironmentNotations
+       SamplesNotations RContextNotations.
+
+(** * Transition - Temporal - Definition
+
+Wormholes’s semantics is given by three sets of transition rules: the evaluation
+transition, which extends standard β-reduction; the functional transition which
+performs the logical instant, and the temporal transition which corresponds to
+the reactivity of the program: it initializes the resources values, performs the
+instant via functional transition and updates the system.
+
+In this file, we focus on the temporal transition.
+*)
+
+(** ** Temporal Transition *)
 
 Definition temporal (S S1 : 𝐒) (P P' : Λ) (W W1 : 𝐖) :=
-  forall Vin Vout Wnew _tv,
+  exists (Vin Vout : 𝓥) Wnew _tv,
     (Vin = Stock.init_virtual W (Samples.nexts S))%re /\
                     
     ⪡ Vin ; unit ; P ⪢ ⭆ ⪡ Vout ; _tv ; P' ; Wnew ⪢ /\
                     
-    (S1 = Samples.puts Vout S) /\ (W1 = Stock.update Wnew Vout)%sk. 
+    (S1 = Samples.puts Vout ([⧐ᵣₔ (Vin⁺ᵣᵦ) ≤ (Vout⁺ᵣᵦ - Vin⁺ᵣᵦ)] S))%rf /\ 
+    (W1 = Stock.update Wnew Vout)%sk. 
 
 Notation "'⟦' S ';' W ';' P '⟧' '⟾' '⟦' S1 ';' W1 ';' P1 '⟧'" 
   := (temporal S S1 P P1 W W1) (at level 30, S constr, S1 constr,
@@ -17,4 +31,6 @@ Notation "'⟦' S ';' W ';' P '⟧' '⟾' '⟦' S1 ';' W1 ';' P1 '⟧'"
                                              W constr, W1 constr, no associativity).
 
 
-*)
+Definition wf_env_tT (Re : ℜ) (S : 𝐒) (W : 𝐖) := True.
+
+Notation "'Wfₜₜ(' Re , Sa , W )" := (wf_env_tT Re Sa W) (at level 50).
