theories/Transition/Temporal/TT_Preservation.v
@@ -1,0 +1,62 @@
+From Coq Require Import Relations.Relation_Operators.
+From Mecha Require Import Resource Term ReadStock WriteStock Stock REnvironment
+                          Sample Samples RContext VContext Typing Typ
+                          ET_Definition ET_Preservation FT_Definition FT_Props 
+                          FT_Preservation TT_Definition TT_Props.
+Import ResourceNotations TermNotations StockNotations REnvironmentNotations
+       SamplesNotations RContextNotations VContextNotations TypNotations.
+
+Section preservation.
+
+Hypothesis all_arrow_halting : forall Re t α β,
+  ∅ᵥᵪ ⋅ Re ⊫ arr(t) ∈ (α ⟿ β ∣ ∅ᵣₛ) -> forall v, ∅ᵥᵪ ⋅ Re ⊫ v ∈ α -> halts (Re⁺ᵣᵪ) <[t v]>.
+
+Theorem temporal_preserves_typing (Re : ℜ) (Sa Sa' : 𝐒) (W W' : 𝐖) (P P' : Λ) (R : resources) :
+
+    (* (1) *) halts (Re⁺ᵣᵪ) P -> (* (2) *) Samples.halts (Re⁺ᵣᵪ) Sa -> Stock.halts (Re⁺ᵣᵪ) W ->
+              Wfₜₜ(Re,Sa,W) ->
+
+    (* (1) *) ∅ᵥᵪ ⋅ Re ⊫ P ∈ (𝟙 ⟿ 𝟙 ∣ R) ->
+    (* (3) *) ⟦ Sa ; W ; P ⟧ ⟾ ⟦ Sa' ; W' ; P' ⟧ ->
+
+(*----------------------------------------------------*)
+   exists Re1 R1,
+    (R ⊆ R1)%rs /\ Re ⊆ᵣᵪ Re1 /\
+    ∅ᵥᵪ ⋅ Re1 ⊫ P' ∈ (𝟙 ⟿ 𝟙 ∣ R1) /\ 
+    Wfₜₜ(Re1,Sa',W') /\ 
+    (* (7) *) halts (Re1⁺ᵣᵪ) P' /\ (* (8) *) Samples.halts (Re1⁺ᵣᵪ) Sa' /\ Stock.halts (Re1⁺ᵣᵪ) W'.
+Proof.
+  intros HlP HlSa HlW HwfTT HwP HTT.
+  destruct HTT as [Vin [Vout [Wnew [_tv [HeqVin [fT [HeqSa' HeqW']]]]]]].
+
+  move Vin before R; move Vout before Vin; move Wnew before W'; move _tv before P'.
+  move fT before HwP.
+
+  apply wf_env_TT_to_fT in HwfTT as HwfFT.
+  rewrite <- HeqVin in HwfFT.
+
+  apply (functional_preserves_typing_gen 
+              all_arrow_halting Re _ _ _ _ _ _ _ Typ.ty_unit Typ.ty_unit R) 
+              in fT as IH; 
+  auto.
+  - destruct IH as 
+    [Hunsd [Hunc [Re1 [R1 [HsubRe [HsubR [HwfFT1 
+    [HwtW [HW [Husd [_ [HwtP' [HlP' [_ [HlVout HlWnew]]]]]]]]]]]]]]].
+    exists Re1; exists R1.
+    split; auto; split; auto; split; auto.
+    split.
+    -- admit.
+    -- split; auto; split.
+       + rewrite HeqSa'. apply Samples.halts_puts; auto.
+         rewrite <- (wf_env_fT_new Re Vin HwfFT).
+         rewrite <- (wf_env_fT_new Re1 Vout HwfFT1).
+         apply Samples.halts_weakening; auto.
+         apply RContext.Ext.new_key_Submap_spec; assumption.
+       + rewrite HeqW'. apply Stock.halts_update; auto.
+  - exists <[unit]>; split; auto; apply rt1n_refl.
+  - rewrite HeqVin. apply Stock.halts_init_virtual; auto.
+    now apply Samples.halts_nexts.
+  - constructor.
+Admitted.
+
+End preservation.
