theories/Transition/Temporal/TT_Props.v
@@ -1,0 +1,44 @@
+From Mecha Require Import Resource Term ReadStock WriteStock Stock REnvironment
+                          Sample Samples RContext VContext Typing Typ
+                          ET_Definition ET_Preservation FT_Definition FT_Props TT_Definition.
+Import ResourceNotations TermNotations StockNotations REnvironmentNotations
+       SamplesNotations RContextNotations VContextNotations TypNotations.
+
+Module RE := REnvironment.
+
+
+(** * Transition - Temporal - Properties *)
+
+Lemma resource_used_init_unused : forall Re t α β R W Sa V,
+  ∅ᵥᵪ ⋅ Re ⊫ t ∈ (α ⟿ β ∣ R) ->
+  halts (Re⁺ᵣᵪ) t ->
+  Wfᵣₜ(Re,V) ->
+  (V = Stock.init_virtual W (Samples.nexts Sa))%re ->
+  
+  (forall r, (r ∈ R)%rs -> RE.unused r V).
+Proof.
+  intros Re t α β R W Sa V Hwt Hlt Hwf Heq r HInR.
+  destruct Hlt as [t' [HmeT Hvt']].
+  apply multi_preserves_typing with (t' := t') in Hwt; auto.
+  - apply typing_Re_R with (r := r) in Hwt as HInRe; auto.
+    rewrite (wf_env_fT_in Re V Hwf) in HInRe.
+    rewrite Heq in *. 
+    destruct HInRe as [v HfV].
+    apply RE.OP.P.find_1 in HfV.
+    apply Stock.init_virtual_unused_1 in HfV as Hunsd.
+    -- destruct v; simpl in *.
+       + now exists λ.
+       + contradiction.
+    -- intros r1 v1 HfSa.
+       assert (r1 ∈ᵣₔ Sa). 
+       { rewrite Samples.nexts_in_iff. exists v1. now apply RE.OP.P.find_2. }
+       apply Samples.nexts_unused in H; destruct H.
+       apply RE.OP.P.find_2 in HfSa, H. 
+       eapply RE.OP.P.mapsto_fun in HfSa; eauto.
+       subst; now simpl.
+  - eapply (wf_env_fT_valid Re V Hwf). 
+Qed.
+
+Lemma wf_env_TT_to_fT Re Sa W : 
+  Wfₜₜ(Re,Sa,W) -> Wfᵣₜ(Re,Stock.init_virtual W (Samples.nexts Sa)).
+Proof. Admitted.
