theories/Typing.v
@@ -1,5 +1,5 @@
 From Coq Require Import Lia Arith.PeanoNat Program Bool.Bool Classes.Morphisms.
-From Mecha Require Import Typ Resource Resources Term Var VContext RContext.
+From Mecha Require Import Typ Resource Term Var VContext RContext.
 Import ResourceNotations TypNotations TermNotations RContextNotations VContextNotations.
 
 
